Embedding equivalence in both directions including uniqueness.
Signed-off-by: David Cock <david.cock@inf.ethz.ch>

SimplEmbedding.thy
@@ -29,6 +29,100 @@ primrec embedSimpl :: "('s, 'p, 'f) Language.com \<Rightarrow> ('s, 'p, 'f) OG_L
   | "embedSimpl Language.com.Throw = OG_Language.com.Throw"
   | "embedSimpl (Language.com.Catch a b) = OG_Language.com.Catch (embedSimpl a) (embedSimpl b)"
 
+lemma embedSimpl_inj:
+  "inj embedSimpl"
+proof(rule injI)
+  fix c1 c2::"('s,'p,'f) Language.com"
+  assume "embedSimpl c1 = embedSimpl c2"
+  thus "c1 = c2"
+  proof(induct c1 arbitrary:c2)
+    case Skip
+    then show ?case by(cases c2, auto)
+  next
+    case (Basic f)
+    then show ?case by(cases c2, auto)
+  next
+    case (Spec r)
+    then show ?case by(cases c2, auto)
+  next
+    case (Seq c11 c12)
+    then show ?case by(cases c2, auto)
+  next
+    case (Cond b c11 c12)
+    then show ?case by(cases c2, auto)
+  next
+    case (While b c)
+    then show ?case by(cases c2, auto)
+  next
+    case (Call p)
+    then show ?case by(cases c2, auto)
+  next
+    case (DynCom c)
+    note outer = this
+    then show ?case
+    proof(cases c2)
+      case Skip
+      with DynCom show ?thesis by(auto)
+    next
+      case (Basic x2)
+      with DynCom show ?thesis by(auto)
+    next
+      case (Spec x3)
+      with DynCom show ?thesis by(auto)
+    next
+      case (Seq x41 x42)
+      with DynCom show ?thesis by(auto)
+    next
+      case (Cond x51 x52 x53)
+      with DynCom show ?thesis by(auto)
+    next
+      case (While x61 x62)
+      with DynCom show ?thesis by(auto)
+    next
+      case (Call x7)
+      with DynCom show ?thesis by(auto)
+    next
+      case (DynCom c')
+      text \<open>This is the only non-trivial case.  The induction hypothesis + extensionality give us
+            equality on the computations: c = c'.\<close>
+      {
+        fix s
+
+        have "embedSimpl (c s) = (embedSimpl o c) s" by(simp)
+        also {
+          from DynCom outer have "OG_Language.DynCom (embedSimpl o c) = OG_Language.DynCom (embedSimpl o c')"
+            by(simp)
+          hence "(embedSimpl o c) s = (embedSimpl o c') s"
+            by(auto)
+        }
+        also have "(embedSimpl o c') s = embedSimpl (c' s)" by(simp)
+        finally have "c s = c' s"
+          using outer by(auto)
+      }
+      hence "c = c'" by(rule ext)
+      with DynCom outer show ?thesis by(simp)
+    next
+      case (Guard x91 x92 x93)
+      with DynCom show ?thesis by(auto)
+    next
+      case Throw
+      with DynCom show ?thesis by(auto)
+    next
+      case (Catch x111 x112)
+      with DynCom show ?thesis by(auto)
+    qed
+  next
+    case (Guard x1 x2a c1)
+    then show ?case by(cases c2, auto)
+  next
+    case Throw
+    then show ?case by(cases c2, auto)
+  next
+    case (Catch c11 c12)
+    then show ?case by(cases c2, auto)
+  qed
+qed
+
 definition embedContext :: "('s,'p,'f) Semantic.body \<Rightarrow> ('s,'p,'f) OG_SmallStep.body"
   where
     "embedContext \<Gamma> = (\<lambda>x. case x of None \<Rightarrow> None | Some c \<Rightarrow> Some (embedSimpl c)) o \<Gamma>"
@@ -42,6 +136,57 @@ function (sequential) stateRel :: "('s, 'f) Semantic.xstate \<Rightarrow> ('s, '
   | "stateRel xs xs_og \<longleftrightarrow> False"
   by(pat_completeness, auto)
 termination by(lexicographic_order)
+
+lemma stateRel_sv_fwd:
+  "single_valuedp stateRel"
+proof(rule single_valuedpI)
+  fix x y z
+  assume rxy: "stateRel x y" and rxz: "stateRel x z"
+  show "y = z"
+  proof(cases x)
+    case (Normal s)
+    from Normal rxy have "y = OG_SmallStep.Normal s" by(cases y, auto)
+    moreover from Normal rxz have "z = OG_SmallStep.Normal s" by(cases z, auto)
+    ultimately show ?thesis by(simp)
+  next
+    case (Abrupt f)
+    with rxy show ?thesis by(auto)
+  next
+    case (Fault f)
+    from Fault rxy have "y = OG_SmallStep.Fault f" by(cases y, auto)
+    moreover from Fault rxz have "z = OG_SmallStep.Fault f" by(cases z, auto)
+    ultimately show ?thesis by(simp)
+  next
+    case Stuck
+    from Stuck rxy have "y = OG_SmallStep.Stuck" by(cases y, auto)
+    moreover from Stuck rxz have "z = OG_SmallStep.Stuck" by(cases z, auto)
+    ultimately show ?thesis by(simp)
+  qed
+qed
+
+lemma stateRel_sv_rev:
+  "single_valuedp (conversep stateRel)"
+proof(rule single_valuedpI)
+  fix x y z
+  assume rxy: "(conversep stateRel) x y" and rxz: "(conversep stateRel) x z"
+  show "y = z"
+  proof(cases x)
+    case (Normal s)
+    from Normal rxy have "y = Semantic.Normal s" by(cases y, auto)
+    moreover from Normal rxz have "z = Semantic.Normal s" by(cases z, auto)
+    ultimately show ?thesis by(simp)
+  next
+    case (Fault f)
+    from Fault rxy have "y = Semantic.Fault f" by(cases y, auto)
+    moreover from Fault rxz have "z = Semantic.Fault f" by(cases z, auto)
+    ultimately show ?thesis by(simp)
+  next
+    case Stuck
+    from Stuck rxy have "y = Semantic.Stuck" by(cases y, auto)
+    moreover from Stuck rxz have "z = Semantic.Stuck" by(cases z, auto)
+    ultimately show ?thesis by(simp)
+  qed
+qed
 
 lemma stateRel_fw_Normal:
   "stateRel (Semantic.Normal s) xs_og \<Longrightarrow> xs_og = OG_SmallStep.Normal s"
@@ -77,48 +222,33 @@ lemmas stateRel_rewrites =
   stateRel_fw_Stuck stateRel_rev_Stuck
   stateRel_no_Abrupt
 
-definition wf_com :: "('s, 'p, 'f) Language.com \<Rightarrow> bool"
-  where "wf_com c = True"
-
-lemma wf_comI: "wf_com c" by(simp add:wf_com_def)
-
-thm OG_SmallStep.step_elim_cases
-
-lemma final_cases:
-  assumes "OG_SmallStep.final (c,xs)"
-  obtains (Skip) "c = OG_Language.Skip" | 
-          (Throw) s where "c = OG_Language.Throw" and "xs = OG_SmallStep.Normal s"
-  using assms unfolding final_def by(auto)
-
-primrec og_com_size :: "('s,'p,'f) OG_Language.com \<Rightarrow> nat"
-  where "og_com_size Skip = 1" |
-        "og_com_size (Basic f) = 1" |
-        "og_com_size (Spec r) = 1" |
-        "og_com_size (Seq c1 c2) = og_com_size c1 + og_com_size c2 + 1" |
-        "og_com_size (Cond b c1 c2) = og_com_size c1 + og_com_size c2 + 1" |
-        "og_com_size (While b c) = og_com_size c + 1" |
-        "og_com_size (Call p) = 1" |
-        "og_com_size (DynCom d) = 1" |
-        "og_com_size (Guard f g c) = og_com_size c + 1" |
-        "og_com_size Throw = 1" |
-        "og_com_size (Catch c1 c2) = og_com_size c1 + og_com_size c2 + 1" |
-        "og_com_size (Parallel s) = (sum_list (map og_com_size s)) + 1" |
-        "og_com_size (Await g c) = og_com_size c + 1"
+primrec com_size :: "('s,'p,'f) Language.com \<Rightarrow> nat"
+  where "com_size Language.Skip = 1" |
+        "com_size (Language.Basic f) = 1" |
+        "com_size (Language.Spec r) = 1" |
+        "com_size (Language.Seq c1 c2) = com_size c1 + com_size c2 + 1" |
+        "com_size (Language.Cond b c1 c2) = com_size c1 + com_size c2 + 1" |
+        "com_size (Language.While b c) = com_size c + 1" |
+        "com_size (Language.Call p) = 1" |
+        "com_size (Language.DynCom d) = 1" |
+        "com_size (Language.Guard f g c) = com_size c + 1" |
+        "com_size Language.Throw = 1" |
+        "com_size (Language.Catch c1 c2) = com_size c1 + com_size c2 + 1"
 
 lemma redex_size_le:
-  "og_com_size (redex c) \<le> og_com_size c"
+  "com_size (SmallStep.redex c) \<le> com_size c"
   by(induct c, auto)
 
 lemma redex_Seq_ne:
   fixes c1 c2
-  shows "redex (Seq c1 c2) \<noteq> Seq c1 c2"
+  shows "SmallStep.redex (Language.Seq c1 c2) \<noteq> Language.Seq c1 c2"
 proof
-  assume "redex (Seq c1 c2) = Seq c1 c2"
-  hence "og_com_size (Seq c1 c2) = og_com_size (redex c1)"
+  assume "SmallStep.redex (Language.Seq c1 c2) = Language.Seq c1 c2"
+  hence "com_size (Language.Seq c1 c2) = com_size (SmallStep.redex c1)"
     by(simp)
-  also from redex_size_le have "... \<le> og_com_size c1"
+  also from redex_size_le have "... \<le> com_size c1"
     by(auto)
-  also have "... < og_com_size (Seq c1 c2)"
+  also have "... < com_size (Language.Seq c1 c2)"
     by(simp)
   finally show False
     by(simp)
@@ -126,14 +256,63 @@ qed
 
 lemma redex_Catch_ne:
   fixes c1 c2
-  shows "redex (Catch c1 c2) \<noteq> Catch c1 c2"
+  shows "SmallStep.redex (Language.Catch c1 c2) \<noteq> Language.Catch c1 c2"
 proof
-  assume "redex (Catch c1 c2) = Catch c1 c2"
-  hence "og_com_size (Catch c1 c2) = og_com_size (redex c1)"
+  assume "SmallStep.redex (Language.Catch c1 c2) = Language.Catch c1 c2"
+  hence "com_size (Language.Catch c1 c2) = com_size (SmallStep.redex c1)"
     by(simp)
-  also from redex_size_le have "... \<le> og_com_size c1"
+  also from redex_size_le have "... \<le> com_size c1"
     by(auto)
-  also have "... < og_com_size (Catch c1 c2)"
+  also have "... < com_size (Language.Catch c1 c2)"
+    by(simp)
+  finally show False
+    by(simp)
+qed
+
+primrec og_com_size :: "('s,'p,'f) OG_Language.com \<Rightarrow> nat"
+  where "og_com_size OG_Language.Skip = 1" |
+        "og_com_size (OG_Language.Basic f) = 1" |
+        "og_com_size (OG_Language.Spec r) = 1" |
+        "og_com_size (OG_Language.Seq c1 c2) = og_com_size c1 + og_com_size c2 + 1" |
+        "og_com_size (OG_Language.Cond b c1 c2) = og_com_size c1 + og_com_size c2 + 1" |
+        "og_com_size (OG_Language.While b c) = og_com_size c + 1" |
+        "og_com_size (OG_Language.Call p) = 1" |
+        "og_com_size (OG_Language.DynCom d) = 1" |
+        "og_com_size (OG_Language.Guard f g c) = og_com_size c + 1" |
+        "og_com_size OG_Language.Throw = 1" |
+        "og_com_size (OG_Language.Catch c1 c2) = og_com_size c1 + og_com_size c2 + 1" |
+        "og_com_size (OG_Language.Parallel s) = (sum_list (map og_com_size s)) + 1" |
+        "og_com_size (OG_Language.Await g c) = og_com_size c + 1"
+
+lemma og_redex_size_le:
+  "og_com_size (OG_SmallStep.redex c) \<le> og_com_size c"
+  by(induct c, auto)
+
+lemma og_redex_Seq_ne:
+  fixes c1 c2
+  shows "OG_SmallStep.redex (OG_Language.Seq c1 c2) \<noteq> OG_Language.Seq c1 c2"
+proof
+  assume "OG_SmallStep.redex (OG_Language.Seq c1 c2) = OG_Language.Seq c1 c2"
+  hence "og_com_size (OG_Language.Seq c1 c2) = og_com_size (OG_SmallStep.redex c1)"
+    by(simp)
+  also from og_redex_size_le have "... \<le> og_com_size c1"
+    by(auto)
+  also have "... < og_com_size (OG_Language.Seq c1 c2)"
+    by(simp)
+  finally show False
+    by(simp)
+qed
+
+lemma og_redex_Catch_ne:
+  fixes c1 c2
+  shows "OG_SmallStep.redex (OG_Language.Catch c1 c2) \<noteq> OG_Language.Catch c1 c2"
+proof
+  assume "OG_SmallStep.redex (OG_Language.Catch c1 c2) = OG_Language.Catch c1 c2"
+  hence "og_com_size (OG_Language.Catch c1 c2) = og_com_size (OG_SmallStep.redex c1)"
+    by(simp)
+  also from og_redex_size_le have "... \<le> og_com_size c1"
+    by(auto)
+  also have "... < og_com_size (OG_Language.Catch c1 c2)"
     by(simp)
   finally show False
     by(simp)
@@ -148,7 +327,7 @@ lemma embedSimpl_fwd_refine:
   using embed_step
 proof(induct c arbitrary:c_og' xs_og')
   case Skip
-  with embed_step show ?case
+  thus ?case
     by(auto intro:OG_SmallStep.no_step_final[unfolded OG_SmallStep.final_def])
 next
   case (Basic f)
@@ -278,10 +457,10 @@ next
     ultimately show ?thesis by(blast)
   next
     case (4 f)
-    with redex_Seq_ne show ?thesis by(blast)
+    with og_redex_Seq_ne show ?thesis by(blast)
   next
     case 5
-    with redex_Seq_ne show ?thesis by(blast)
+    with og_redex_Seq_ne show ?thesis by(blast)
   qed
 
 next
@@ -582,11 +761,33 @@ next
     ultimately show ?thesis by(blast)
   next
     case (4 f)
-    with redex_Catch_ne show ?thesis by(blast)
+    with og_redex_Catch_ne show ?thesis by(blast)
   next
     case 5
-    with redex_Catch_ne show ?thesis by(blast)
+    with og_redex_Catch_ne show ?thesis by(blast)
   qed
+qed
+
+text \<open>The forward embedding is single-valued.\<close>
+lemma embedSimpl_fwd_refine1:
+  assumes sr: "stateRel xs xs_og"
+      and embed_step: "OG_SmallStep.step (embedContext \<Gamma>) (embedSimpl c, xs_og) (c_og', xs_og')"
+    shows "\<exists>!(c',xs'). c_og' = embedSimpl c' \<and> SmallStep.step \<Gamma> (c, xs) (c', xs') \<and> stateRel xs' xs_og'"
+      (is "\<exists>!(c',xs'). ?P c' \<and> ?Q c' xs' \<and> ?R xs'")
+proof -
+  from embedSimpl_fwd_refine[OF assms] have "\<exists>c' xs'. ?P c' \<and> ?Q c' xs' \<and> ?R xs'"
+    by(blast)
+  moreover {
+    fix c' xs' c'' xs''
+    assume P1: "?P c' \<and> ?Q c' xs' \<and> ?R xs'"
+       and P2: "?P c'' \<and> ?Q c'' xs'' \<and> ?R xs''"
+
+    from embedSimpl_inj P1 P2 have "c' = c''" by(blast dest:inj_eq)
+    moreover from stateRel_sv_rev P1 P2 have "xs' = xs''"
+      unfolding single_valuedp_def by(auto)
+    ultimately have "(c',xs') = (c'',xs'')" by(simp)
+  }
+  ultimately show ?thesis by(auto)
 qed
 
 text \<open>Elimination rule form of forward refinement.\<close>
@@ -598,5 +799,497 @@ lemma embedSimpl_fwdE[consumes 2]:
       and "SmallStep.step \<Gamma> (c, xs) (c', xs')"
       and "stateRel xs' xs_og'"
   using embedSimpl_fwd_refine[OF assms] by(auto)
+
+text \<open>Embedding is faithful - any step of the Simpl program is also a step of the Complx.\<close>
+lemma embedSimpl_rev_refine:
+  assumes sr: "stateRel xs xs_og"
+      and step: "SmallStep.step \<Gamma> (c, xs) (c', xs')"
+    shows "\<exists>xs_og'. OG_SmallStep.step (embedContext \<Gamma>) (embedSimpl c, xs_og) (embedSimpl c', xs_og') \<and> stateRel xs' xs_og'"
+  using step
+proof(induct c arbitrary:c')
+  case Skip
+  thus ?case
+    by(auto intro:SmallStep.no_step_final[unfolded SmallStep.final_def])
+next
+  case (Basic f)
+
+  from Basic show ?case
+  proof(cases rule:SmallStep.step_elim_cases(3))
+    case (1 s)
+    hence "stateRel xs' (OG_SmallStep.Normal (f s))" by(simp)
+    moreover {
+      from 1 sr have "xs_og = OG_SmallStep.Normal s" by(cases xs_og, auto)
+      with 1 have "OG_SmallStep.step (embedContext \<Gamma>) (embedSimpl (Language.Basic f), xs_og)
+                    (embedSimpl c', OG_SmallStep.Normal (f s))"
+        by(auto intro:OG_SmallStep.step.Basic)
+    }
+    ultimately show ?thesis by(blast)
+  next
+    case (2 flt)
+    hence "stateRel xs' (OG_SmallStep.Fault flt)" by(simp)
+    moreover {
+      from 2 sr have "xs_og = OG_SmallStep.Fault flt" by(cases xs_og, auto)
+      with 2 have "OG_SmallStep.step (embedContext \<Gamma>) (embedSimpl (Language.Basic f), xs_og)
+                    (embedSimpl c', OG_SmallStep.Fault flt)"
+        by(auto intro:OG_SmallStep.step.FaultProp)
+    }
+    ultimately show ?thesis by(blast)
+  next
+    case 3
+    hence "stateRel xs' OG_SmallStep.Stuck" by(simp)
+    moreover {
+      from 3 sr have "xs_og = OG_SmallStep.Stuck" by(cases xs_og, auto)
+      with 3 have "OG_SmallStep.step (embedContext \<Gamma>) (embedSimpl (Language.Basic f), xs_og)
+                    (embedSimpl c', OG_SmallStep.Stuck)"
+        by(auto intro:OG_SmallStep.step.StuckProp)
+    }
+    ultimately show ?thesis by(blast)
+  next
+    text \<open>The Abrupt state is forbidden by the state relation.\<close>
+    case (4 f)
+    with sr show ?thesis by(simp)
+  qed
+
+next
+  case (Spec r)
+
+  from Spec show ?case
+  proof(cases rule:SmallStep.step_elim_cases(4))
+    case (1 s t)
+    hence "stateRel xs' (OG_SmallStep.Normal t)" by(simp)
+    moreover {                    
+      from 1 sr have "xs_og = OG_SmallStep.Normal s" by(cases xs_og, auto)
+      with 1 have "OG_SmallStep.step (embedContext \<Gamma>) (embedSimpl (Language.Spec r), xs_og)
+                    (embedSimpl c', OG_SmallStep.Normal t)"
+        by(auto intro:OG_SmallStep.step.Spec)
+    }
+    ultimately show ?thesis by(blast)
+next
+    case (2 s)
+    hence "stateRel xs' (OG_SmallStep.Stuck)" by(simp)
+    moreover {
+      from 2 sr have "xs_og = OG_SmallStep.Normal s" by(cases xs_og, auto)
+      with 2 have "OG_SmallStep.step (embedContext \<Gamma>) (embedSimpl (Language.Spec r), xs_og)
+                    (embedSimpl c', OG_SmallStep.Stuck)"
+        by(auto intro:OG_SmallStep.step.SpecStuck)
+    }
+    ultimately show ?thesis by(blast)
+  next
+    case (3 flt)
+    hence "stateRel xs' (OG_SmallStep.Fault flt)" by(simp)
+    moreover {
+      from 3 sr have "xs_og = OG_SmallStep.Fault flt" by(cases xs_og, auto)
+      with 3 have "OG_SmallStep.step (embedContext \<Gamma>) (embedSimpl (Language.Spec r), xs_og)
+                    (embedSimpl c', OG_SmallStep.Fault flt)"
+        by(auto intro:OG_SmallStep.step.FaultProp)
+    }
+    ultimately show ?thesis by(blast)
+  next
+    case 4
+    hence "stateRel xs' OG_SmallStep.Stuck" by(simp)
+    moreover {
+      from 4 sr have "xs_og = OG_SmallStep.Stuck" by(cases xs_og, auto)
+      with 4 have "OG_SmallStep.step (embedContext \<Gamma>) (embedSimpl (Language.Spec r), xs_og)
+                    (embedSimpl c', OG_SmallStep.Stuck)"
+        by(auto intro:OG_SmallStep.step.StuckProp)
+    }
+    ultimately show ?thesis by(blast)
+  next
+    case (5 f)
+    with sr show ?thesis by(simp)
+  qed
+
+next
+  case (Seq c1 c2)
+
+  from Seq.prems show ?case
+  proof(cases rule:SmallStep.step_elim_cases(5))
+    case (1 c1' s')
+    with Seq.hyps(1) obtain xs_og'
+        where step_IH: "OG_SmallStep.step (embedContext \<Gamma>) (embedSimpl c1, xs_og) (embedSimpl c1', xs_og')"
+        and sr_IH: "stateRel xs' xs_og'"
+      by(blast)
+
+    from 1 step_IH
+    have "OG_SmallStep.step (embedContext \<Gamma>)
+          (embedSimpl (Language.Seq c1 c2), xs_og) (embedSimpl c', xs_og')"
+      by(auto intro: OG_SmallStep.step.Seq)
+    with sr_IH show ?thesis by(blast)
+  next
+    case 2
+    from 2 sr have "stateRel xs' xs_og" by(simp)
+    moreover {
+      from 2 have "OG_SmallStep.step (embedContext \<Gamma>)
+                    (embedSimpl (Language.Seq c1 c2), xs_og)
+                    (embedSimpl c', xs_og)"
+        by(auto intro:OG_SmallStep.step.SeqSkip)
+    }
+    ultimately show ?thesis by(blast)
+  next
+    case (3 s)
+    from 3 sr have "stateRel xs' (OG_SmallStep.Normal s)" by(simp)
+    moreover {
+      from 3 sr have "xs_og = OG_SmallStep.Normal s" by(cases xs_og, auto)
+      with 3 have "OG_SmallStep.step (embedContext \<Gamma>)
+                    (embedSimpl (Language.Seq c1 c2), xs_og)
+                    (embedSimpl c', OG_SmallStep.Normal s)"
+        by(auto intro:OG_SmallStep.step.SeqThrow)
+    }
+    ultimately show ?thesis by(blast)
+  next
+    case (4 flt)
+    with redex_Seq_ne show ?thesis by(blast)
+  next
+    case 5
+    with redex_Seq_ne show ?thesis by(blast)
+  next
+    case (6 f)
+    with sr show ?thesis by(simp)
+  qed
+
+next
+  case (Cond b c1 c2)
+
+  from Cond.prems show ?case
+  proof(cases rule:SmallStep.step_elim_cases(6))
+    case (1 s)
+    hence "stateRel xs' (OG_SmallStep.Normal s)" by(simp)
+    moreover {
+      from 1 sr have "xs_og = OG_SmallStep.Normal s" by(cases xs_og, auto)
+      with 1 have "OG_SmallStep.step (embedContext \<Gamma>) (embedSimpl (Language.Cond b c1 c2), xs_og)
+                    (embedSimpl c', OG_SmallStep.Normal s)"
+        by(auto intro:OG_SmallStep.step.CondTrue)
+    }
+    ultimately show ?thesis by(blast)
+  next
+    case (2 s)
+    hence "stateRel xs' (OG_SmallStep.Normal s)" by(simp)
+    moreover {
+      from 2 sr have "xs_og = OG_SmallStep.Normal s" by(cases xs_og, auto)
+      with 2 have "OG_SmallStep.step (embedContext \<Gamma>) (embedSimpl (Language.Cond b c1 c2), xs_og)
+                    (embedSimpl c', OG_SmallStep.Normal s)"
+        by(auto intro:OG_SmallStep.step.CondFalse)
+    }
+    ultimately show ?thesis by(blast)
+  next
+    case (3 flt)
+    hence "stateRel xs' (OG_SmallStep.Fault flt)" by(simp)
+    moreover {
+      from 3 sr have "xs_og = OG_SmallStep.Fault flt" by(cases xs_og, auto)
+      with 3 have "OG_SmallStep.step (embedContext \<Gamma>) (embedSimpl (Language.Cond b c1 c2), xs_og)
+                    (embedSimpl c', OG_SmallStep.Fault flt)"
+        by(auto intro:OG_SmallStep.step.FaultProp)
+    }
+    ultimately show ?thesis by(blast)
+  next
+    case 4
+    hence "stateRel xs' OG_SmallStep.Stuck" by(simp)
+    moreover {
+      from 4 sr have "xs_og = OG_SmallStep.Stuck" by(cases xs_og, auto)
+      with 4 have "OG_SmallStep.step (embedContext \<Gamma>) (embedSimpl (Language.Cond b c1 c2), xs_og)
+                    (embedSimpl c', OG_SmallStep.Stuck)"
+        by(auto intro:OG_SmallStep.step.StuckProp)
+    }
+    ultimately show ?thesis by(blast)
+  next
+    case (5 f)
+    with sr show ?thesis by(simp)
+  qed
+
+next
+  case (While b c)
+
+  from While.prems show ?case
+  proof(cases rule:SmallStep.step_elim_cases(7))
+    case (1 s)
+    hence "stateRel xs' (OG_SmallStep.Normal s)" by(simp)
+    moreover {
+      from 1 sr have "xs_og = OG_SmallStep.Normal s" by(cases xs_og, auto)
+      with 1 have "OG_SmallStep.step (embedContext \<Gamma>) (embedSimpl (Language.While b c), xs_og)
+                    (embedSimpl c', OG_SmallStep.Normal s)"
+        by(auto intro:OG_SmallStep.step.WhileTrue)
+    }
+    ultimately show ?thesis by(blast)
+  next
+    case (2 s)
+    hence "stateRel xs' (OG_SmallStep.Normal s)" by(simp)
+    moreover {
+      from 2 sr have "xs_og = OG_SmallStep.Normal s" by(cases xs_og, auto)
+      with 2 have "OG_SmallStep.step (embedContext \<Gamma>) (embedSimpl (Language.While b c), xs_og)
+                    (embedSimpl c', OG_SmallStep.Normal s)"
+        by(auto intro:OG_SmallStep.step.WhileFalse)
+    }
+    ultimately show ?thesis by(blast)
+  next
+    case (3 flt)
+    hence "stateRel xs' (OG_SmallStep.Fault flt)" by(simp)
+    moreover {
+      from 3 sr have "xs_og = OG_SmallStep.Fault flt" by(cases xs_og, auto)
+      with 3 have "OG_SmallStep.step (embedContext \<Gamma>) (embedSimpl (Language.While b c), xs_og)
+                    (embedSimpl c', OG_SmallStep.Fault flt)"
+        by(auto intro:OG_SmallStep.step.FaultProp)
+    }
+    ultimately show ?thesis by(blast)
+  next
+    case 4
+    hence "stateRel xs' OG_SmallStep.Stuck" by(simp)
+    moreover {
+      from 4 sr have "xs_og = OG_SmallStep.Stuck" by(cases xs_og, auto)
+      with 4 have "OG_SmallStep.step (embedContext \<Gamma>) (embedSimpl (Language.While b c), xs_og)
+                    (embedSimpl c', OG_SmallStep.Stuck)"
+        by(auto intro:OG_SmallStep.step.StuckProp)
+    }
+    ultimately show ?thesis by(blast)
+  next
+    case (5 f)
+    with sr show ?thesis by(simp)
+  qed
+
+next
+  case (Call p)
+
+  from Call.prems show ?case
+  proof(cases rule:SmallStep.step_elim_cases(8))
+    case (1 bdy s)
+    hence lookup: "(embedContext \<Gamma>) p = Some (embedSimpl bdy)"
+      unfolding embedContext_def by(simp)
+    from 1 have "stateRel xs' (OG_SmallStep.Normal s)" by(simp)
+    moreover {
+      from 1 sr have "xs_og = OG_SmallStep.Normal s" by(cases xs_og, auto)
+      with 1 lookup
+      have "OG_SmallStep.step (embedContext \<Gamma>)
+              (embedSimpl (Language.Call p), xs_og)
+              (embedSimpl c', OG_SmallStep.Normal s)"
+        by(auto intro:OG_SmallStep.step.Call)
+    }
+    ultimately show ?thesis by(blast)
+  next
+    case (2 s)
+    hence lookup: "(embedContext \<Gamma>) p = None"
+      unfolding embedContext_def by(simp)
+    from 2 have "stateRel xs' OG_SmallStep.Stuck" by(simp)
+    moreover {
+      from 2 sr have "xs_og = OG_SmallStep.Normal s" by(cases xs_og, auto)
+      with 2 lookup
+      have "OG_SmallStep.step (embedContext \<Gamma>)
+              (embedSimpl (Language.Call p), xs_og)
+              (embedSimpl c', OG_SmallStep.Stuck)"
+        by(auto intro:OG_SmallStep.step.CallUndefined)
+    }
+    ultimately show ?thesis by(blast)
+  next
+    case (3 flt)
+    hence "stateRel xs' (OG_SmallStep.Fault flt)" by(simp)
+    moreover {
+      from 3 sr have "xs_og = OG_SmallStep.Fault flt" by(cases xs_og, auto)
+      with 3 have "OG_SmallStep.step (embedContext \<Gamma>) (embedSimpl (Language.Call p), xs_og)
+                    (embedSimpl c', OG_SmallStep.Fault flt)"
+        by(auto intro:OG_SmallStep.step.FaultProp)
+    }
+    ultimately show ?thesis by(blast)
+  next
+    case 4
+    hence "stateRel xs' OG_SmallStep.Stuck" by(simp)
+    moreover {
+      from 4 sr have "xs_og = OG_SmallStep.Stuck" by(cases xs_og, auto)
+      with 4 have "OG_SmallStep.step (embedContext \<Gamma>) (embedSimpl (Language.Call p), xs_og)
+                    (embedSimpl c', OG_SmallStep.Stuck)"
+        by(auto intro:OG_SmallStep.step.StuckProp)
+    }
+    ultimately show ?thesis by(blast)
+  next
+    case (5 f)
+    with sr show ?thesis by(simp)
+  qed
+
+next
+  case (DynCom c)
+
+  from DynCom.prems show ?case
+  proof(cases rule:SmallStep.step_elim_cases(9))
+    case (1 s)
+    hence "stateRel xs' (OG_SmallStep.Normal s)" by(simp)
+    moreover {
+      from 1 sr have "xs_og = OG_SmallStep.Normal s" by(cases xs_og, auto)
+      with 1 have "OG_SmallStep.step (embedContext \<Gamma>) (embedSimpl (Language.DynCom c), xs_og)
+                    (embedSimpl c', OG_SmallStep.Normal s)"
+        by(auto intro:OG_SmallStep.step.DynCom simp:o_def)
+      }
+    ultimately show ?thesis by(blast)
+  next
+    case (2 flt)
+    hence "stateRel xs' (OG_SmallStep.Fault flt)" by(simp)
+    moreover {
+      from 2 sr have "xs_og = OG_SmallStep.Fault flt" by(cases xs_og, auto)
+      with 2 have "OG_SmallStep.step (embedContext \<Gamma>) (embedSimpl (Language.DynCom c), xs_og)
+                    (embedSimpl c', OG_SmallStep.Fault flt)"
+        by(auto intro:OG_SmallStep.step.FaultProp)
+    }
+    ultimately show ?thesis by(blast)
+  next
+    case 3
+    hence "stateRel xs' OG_SmallStep.Stuck" by(simp)
+    moreover {
+      from 3 sr have "xs_og = OG_SmallStep.Stuck" by(cases xs_og, auto)
+      with 3 have "OG_SmallStep.step (embedContext \<Gamma>) (embedSimpl (Language.DynCom c), xs_og)
+                    (embedSimpl c', OG_SmallStep.Stuck)"
+        by(auto intro:OG_SmallStep.step.StuckProp)
+    }
+    ultimately show ?thesis by(blast)
+  next
+    case (4 f)
+    with sr show ?thesis by(simp)
+  qed
+
+next
+  case (Guard f g c)
+
+  from Guard.prems show ?case
+  proof(cases rule:SmallStep.step_elim_cases(2))
+    case (1 s)
+    hence "stateRel xs' (OG_SmallStep.Normal s)" by(simp)
+    moreover {
+      from 1 sr have "xs_og = OG_SmallStep.Normal s" by(cases xs_og, auto)
+      with 1 have "OG_SmallStep.step (embedContext \<Gamma>) (embedSimpl (Language.Guard f g c), xs_og)
+                    (embedSimpl c', OG_SmallStep.Normal s)"
+        by(auto intro:OG_SmallStep.step.Guard)
+    }
+    ultimately show ?thesis by(blast)
+  next
+    case (2 s)
+    hence "stateRel xs' (OG_SmallStep.Fault f)" by(simp)
+    moreover {
+      from 2 sr have "xs_og = OG_SmallStep.Normal s" by(cases xs_og, auto)
+      with 2 have "OG_SmallStep.step (embedContext \<Gamma>) (embedSimpl (Language.Guard f g c), xs_og)
+                    (embedSimpl c', OG_SmallStep.Fault f)"
+        by(auto intro:OG_SmallStep.step.GuardFault)
+    }
+    ultimately show ?thesis by(blast)
+  next
+    case (3 flt)
+    hence "stateRel xs' (OG_SmallStep.Fault flt)" by(simp)
+    moreover {
+      from 3 sr have "xs_og = OG_SmallStep.Fault flt" by(cases xs_og, auto)
+      with 3 have "OG_SmallStep.step (embedContext \<Gamma>) (embedSimpl (Language.Guard f g c), xs_og)
+                    (embedSimpl c', OG_SmallStep.Fault flt)"
+        by(auto intro:OG_SmallStep.step.FaultProp)
+    }
+    ultimately show ?thesis by(blast)
+  next
+    case 4
+    hence "stateRel xs' OG_SmallStep.Stuck" by(simp)
+    moreover {
+      from 4 sr have "xs_og = OG_SmallStep.Stuck" by(cases xs_og, auto)
+      with 4 have "OG_SmallStep.step (embedContext \<Gamma>) (embedSimpl (Language.Guard f g c), xs_og)
+                    (embedSimpl c', OG_SmallStep.Stuck)"
+        by(auto intro:OG_SmallStep.step.StuckProp)
+    }
+    ultimately show ?thesis by(blast)
+  next
+    case (5 f)
+    with sr show ?thesis by(simp)
+  qed
+
+next
+  case Throw
+
+  from Throw.prems show ?case
+  proof(cases rule:SmallStep.step_elim_cases(10))
+    case (1 f)
+    hence "stateRel xs' (OG_SmallStep.Fault f)" by(simp)
+    moreover {
+      from 1 sr have "xs_og = OG_SmallStep.Fault f" by(cases xs_og, auto)
+      with 1 have "OG_SmallStep.step (embedContext \<Gamma>) (embedSimpl Language.Throw, xs_og)
+                    (embedSimpl c', OG_SmallStep.Fault f)"
+        by(auto intro:OG_SmallStep.step.FaultProp)
+    }
+    ultimately show ?thesis by(blast)
+  next
+    case 2
+    hence "stateRel xs' OG_SmallStep.Stuck" by(simp)
+    moreover {
+      from 2 sr have "xs_og = OG_SmallStep.Stuck" by(cases xs_og, auto)
+      with 2 have "OG_SmallStep.step (embedContext \<Gamma>) (embedSimpl Language.Throw, xs_og)
+                    (embedSimpl c', OG_SmallStep.Stuck)"
+        by(auto intro:OG_SmallStep.step.StuckProp)
+    }
+    ultimately show ?thesis by(blast)
+  next
+    case (3 f)
+    with sr show ?thesis by(simp)
+  qed
+
+next
+  case (Catch c1 c2)
+
+  from Catch.prems show ?case
+  proof(cases rule:SmallStep.step_elim_cases(11))
+    case (1 c1' s')
+    with Catch.hyps(1) obtain xs_og'
+        where step_IH: "OG_SmallStep.step (embedContext \<Gamma>) (embedSimpl c1, xs_og) (embedSimpl c1', xs_og')"
+        and sr_IH: "stateRel xs' xs_og'"
+      by(blast)
+
+    from 1 step_IH
+    have "OG_SmallStep.step (embedContext \<Gamma>)
+          (embedSimpl (Language.Catch c1 c2), xs_og) (embedSimpl c', xs_og')"
+      by(auto intro: OG_SmallStep.step.Catch)
+    with sr_IH show ?thesis by(blast)
+  next
+    case (2 s)
+    with sr have "stateRel xs' xs_og" by(simp)
+    moreover {
+      from 2 sr have "xs_og = OG_SmallStep.Normal s" by(cases xs_og, auto)
+      with 2 have "OG_SmallStep.step (embedContext \<Gamma>) (embedSimpl (Language.Catch c1 c2), xs_og)
+                    (embedSimpl c', xs_og)"
+        by(auto intro:OG_SmallStep.step.CatchThrow)
+    }
+    ultimately show ?thesis by(blast)
+next
+    case 3
+    with sr have "stateRel xs' xs_og" by(simp)
+    moreover
+    from 3 have "OG_SmallStep.step (embedContext \<Gamma>) (embedSimpl (Language.Catch c1 c2), xs_og)
+                  (embedSimpl c', xs_og)"
+     by(auto intro:OG_SmallStep.step.CatchSkip)
+    ultimately show ?thesis by(blast)
+  next
+    case (4 f)
+    with redex_Catch_ne show ?thesis by(blast)
+  next
+    case 5
+    with redex_Catch_ne show ?thesis by(blast)
+  next
+    case (6 f)
+    with sr show ?thesis by(simp)
+  qed
+qed
+
+text \<open>The reverse refinement is also unique.  It's functional in both directions.\<close>
+lemma embedSimpl_rev_refine1:
+  assumes sr: "stateRel xs xs_og"
+      and step: "SmallStep.step \<Gamma> (c, xs) (c', xs')"
+    shows "\<exists>!xs_og'. OG_SmallStep.step (embedContext \<Gamma>) (embedSimpl c, xs_og) (embedSimpl c', xs_og') \<and> stateRel xs' xs_og'"
+      (is "\<exists>!xs_og'. ?P xs_og'")
+proof -
+  from embedSimpl_rev_refine[OF assms] have "\<exists>xs_og'. ?P xs_og'"
+    by(blast)
+  moreover {
+    fix xs_og' xs_og''
+    assume "?P xs_og'" and "?P xs_og''"
+    with stateRel_sv_fwd have "xs_og' = xs_og''"
+      unfolding single_valuedp_def by(auto)
+  }
+  ultimately show ?thesis by(auto)
+qed
+
+text \<open>Elimination rule form of reverse refinement.\<close>
+lemma embedSimpl_revE[consumes 2]:
+  assumes sr: "stateRel xs xs_og"
+      and step: "SmallStep.step \<Gamma> (c, xs) (c', xs')"
+  obtains (Complx) xs_og'
+    where "OG_SmallStep.step (embedContext \<Gamma>) (embedSimpl c, xs_og) (embedSimpl c', xs_og')"
+      and "stateRel xs' xs_og'"
+  using embedSimpl_rev_refine[OF assms] by(auto)
 
 end
